src/datalog/Node.v
@@ -1,0 +1,171 @@
+From Stdlib Require Import List.
+From Datalog Require Import List Datalog Smallstep.
+From coqutil Require Import Map.Interface.
+Import ListNotations.
+
+Section __.
+  Context {rel : relT} {exprvar : exprvarT} {fn : fnT} {aggregator : aggregatorT} {T : valueT}.
+  Context `{sig : signature fn aggregator T}.
+  Context {context : map.map exprvar T} {context_ok : map.ok context}.
+
+  Implicit Types mf_rel : rel.
+  Implicit Types mf_args : list (option T).
+  Implicit Types nf_args : list T.
+
+  Inductive dfact :=
+  | normal_dfact (nf_rel : rel) (nf_args : list T)
+  | meta_dfact (mf_rel : rel) (mf_args : list (option T)) (source : option nat) (expected_msgs : nat).
+
+  Implicit Types known_facts sent_facts waiting_facts input_facts inputs : list dfact.
+  Implicit Types nf result : dfact.
+
+  Record node_state :=
+    { known_facts : list dfact;
+      waiting_facts : list dfact;
+      sent_facts : list dfact }.
+
+  Definition learn_fact_at_rule (s1 s2 : node_state) : Prop :=
+    exists l1 x l2,
+      s2.(known_facts) = x :: s1.(known_facts) /\
+        s1.(waiting_facts) = l1 ++ x :: l2 /\
+        s2.(waiting_facts) = l1 ++ l2 /\
+        s2.(sent_facts) = s1.(sent_facts).
+
+  Context (is_input : rel -> bool).
+  Context (R_senders : rel -> list nat).
+
+  Definition expect_num_R_facts R mf_args known_facts num :=
+    if is_input R then
+      In (meta_dfact R mf_args None num) known_facts
+    else
+      exists expected_msgss,
+        Forall2 (fun n expected_msgs => In (meta_dfact R mf_args (Some n) expected_msgs) known_facts) (R_senders R) expected_msgss /\
+          num = fold_left Nat.add expected_msgss O.
+
+  Definition dfact_matches mf_rel mf_args nf :=
+    exists nf_args,
+      nf = normal_dfact mf_rel nf_args /\
+        Forall2 matches mf_args nf_args.
+
+  Definition knows_datalog_fact (dfacts : list dfact) (f : fact) :=
+    match f with
+    | normal_fact nf_rel nf_args =>
+        In (normal_dfact nf_rel nf_args) dfacts
+    | meta_fact mf_rel mf_args mf_set =>
+        exists num,
+        expect_num_R_facts mf_rel mf_args dfacts num /\
+          Existsn (dfact_matches mf_rel mf_args) num dfacts /\
+          (forall nf_args,
+              Forall2 matches mf_args nf_args ->
+              mf_set nf_args <-> In (normal_dfact mf_rel nf_args) dfacts)
+    end.
+
+  Definition can_deduce_normal_fact (r : rule) (known_facts : list dfact) nf_rel nf_args :=
+    exists hyps,
+      non_meta_rule_impl r nf_rel nf_args hyps /\
+        Forall (knows_datalog_fact known_facts) hyps.
+
+  Definition can_deduce_meta_fact (mf_concls mf_hyps : list meta_clause) (node: nat) (sent_facts : list dfact) (result : dfact) (hyps : list fact) :=
+    exists ctx mf_rel mf_args mf_cnt,
+      result = meta_dfact mf_rel mf_args (Some node) mf_cnt /\
+        Existsn (dfact_matches mf_rel mf_args) mf_cnt sent_facts /\
+        Exists (fun c => interp_meta_clause ctx c (meta_fact mf_rel mf_args (fun _ => False))) mf_concls /\
+        Forall2 (interp_meta_clause ctx) mf_hyps hyps.
+
+  Definition ok_to_deduce_fact (r : rule) known sent f :=
+    match f with
+    | normal_dfact nf_rel nf_args => True
+    | meta_dfact mf_rel mf_args source num_msgs =>
+        forall nf_args,
+          can_deduce_normal_fact r known mf_rel nf_args ->
+          Forall2 matches mf_args nf_args ->
+          In (normal_dfact mf_rel nf_args) sent
+    end.
+
+  Definition can_deduce_fact (r : rule) node known sent f :=
+    match f with
+    | normal_dfact nf_rel nf_args =>
+        can_deduce_normal_fact r known nf_rel nf_args /\
+          forall mf_args num,
+            In (meta_dfact nf_rel mf_args (Some node) num) sent ->
+            Forall2 matches mf_args nf_args ->
+            False
+    | meta_dfact mf_rel mf_args source num_msgs =>
+        source = Some node /\
+          exists mr_concls mr_hyps hyps,
+            r = meta_rule mr_concls mr_hyps /\
+              can_deduce_meta_fact mr_concls mr_hyps node sent f hyps /\
+              Forall (knows_datalog_fact known) hyps
+    end.
+
+  Record spec_node_prog :=
+    { spec_node_rules : list rule;
+      spec_node_label : nat }.
+
+  Definition new_facts (sp : spec_node_prog) (rs : node_state) f :=
+    Exists
+      (fun r => can_deduce_fact r sp.(spec_node_label) rs.(known_facts) rs.(sent_facts) f)
+      sp.(spec_node_rules) /\
+      Forall
+        (fun r => ok_to_deduce_fact r rs.(known_facts) rs.(sent_facts) f)
+        sp.(spec_node_rules).
+
+  Variant spec_label :=
+    | sl_dequeue
+    | sl_deduce (f : dfact).
+
+  Local Notation IO_event := (Smallstep.IO_event spec_label dfact).
+
+  Inductive spec_node_step (sp : spec_node_prog) : node_state -> IO_event -> node_state -> Prop :=
+  | spec_node_dequeue_step rs input rest :
+    rs.(waiting_facts) = input :: rest ->
+    spec_node_step sp rs (O_event sl_dequeue [])
+                   {| known_facts := input :: rs.(known_facts);
+                     waiting_facts := rest;
+                     sent_facts := rs.(sent_facts) |}
+  | spec_node_deduce_step rs output :
+    new_facts sp rs output ->
+    spec_node_step sp rs (O_event (sl_deduce output) [output])
+                   {| known_facts := rs.(known_facts);
+                     waiting_facts := rs.(waiting_facts);
+                     sent_facts := output :: rs.(sent_facts) |}
+  | spec_node_input_step rs input :
+    spec_node_step sp rs (I_event input)
+                   {| known_facts := rs.(known_facts);
+                     waiting_facts := rs.(waiting_facts) ++ [input];
+                     sent_facts := rs.(sent_facts) |}.
+
+  Definition consistent_inputs (input_facts : list dfact) : Prop :=
+    (forall R mf_args num,
+        In (meta_dfact R mf_args None num) input_facts ->
+        (forall num0, In (meta_dfact R mf_args None num0) input_facts -> num0 = num) /\
+          exists num', num' <= num /\ Existsn (dfact_matches R mf_args) num' input_facts)
+    /\
+    (forall R mf_args k num num0,
+        In (meta_dfact R mf_args (Some k) num) input_facts ->
+        In (meta_dfact R mf_args (Some k) num0) input_facts -> num0 = num)
+    /\
+    (forall R mf_args expected_msgss,
+        Forall2 (fun k e => In (meta_dfact R mf_args (Some k) e) input_facts)
+                (R_senders R) expected_msgss ->
+        exists num', num' <= fold_left Nat.add expected_msgss 0 /\
+                     Existsn (dfact_matches R mf_args) num' input_facts).
+
+  Definition node_allowed (inputs : list dfact) : Prop :=
+    consistent_inputs inputs.
+
+  Definition dfact_equiv (f1 f2 : dfact) : Prop :=
+    match f1, f2 with
+    | meta_dfact R1 a1 s1 _, meta_dfact R2 a2 s2 _ => R1 = R2 /\ a1 = a2 /\ s1 = s2
+    | _, _ => f1 = f2
+    end.
+
+  Definition dfact_consistent (a l : list dfact) : Prop :=
+    forall R margs source num,
+      In (meta_dfact R margs source num) a ->
+      Existsn (dfact_matches R margs) num l.
+
+  Definition node_init : node_state :=
+    {| known_facts := []; waiting_facts := []; sent_facts := [] |}.
+
+End __.
